Working on buffer_changer definition

hello.fst
@@ -1,45 +1,133 @@
 (*--build-config
-options:--admit_fsi FStar.Set;
-other-files:set.fsi heap.fst st.fst all.fst io.fsti string.fst list.fst char.fst;
+options:--admit_fsi FStar.Set --admit_fsi FStar.Heap --admit_fsi FStar.ST --admit_fsi FStar.All --admit_fsi FStar.IO;
+other-files:set.fsi heap.fst st.fst all.fst io.fsti string.fst listTot.fst char.fst terminal.fst;
 --*)
 module Hello
 open FStar.IO
 open FStar.ST
 open FStar.String
-open FStar.List
+open FStar.List.Tot
+open Terminal
 
-val buffer : ref (list (ref string))
-let buffer = ST.alloc [ST.alloc ""]
-let cursor_row = ST.alloc 0
-let cursor_col = ST.alloc 0
+type buffer = (nat * nat * nat * list char)
 
-val str_insert : int -> char -> string -> string
-let str_insert i ch str = strcat (substring str 0 i) (strcat (make 1 ch) (substring str i (strlen str - i)))
+val screen_advance : list char -> terminalScreen -> Tot (option terminalScreen)
+let screen_advance cs scr =
+  let term = Some (StateDefault, scr) in
+  match termChars cs term with
+  | None -> None
+  | Some (state, scr') ->
+    if state = StateDefault then Some scr' else None
 
-val insert_char : char -> ML unit
-let insert_char ch =
-  let sref = nth !buffer !cursor_row in
-  let str = str_insert !cursor_col ch !sref in
-  sref := str
+val pad_list : nat -> 'a -> list 'a -> Tot (list 'a)
+let rec pad_list n v xs' = match n with
+  | 0 -> []
+  | _ -> match xs' with
+    | [] -> v :: pad_list (n-1) v []
+    | x::xs -> x :: pad_list (n-1) v xs
 
-val print_lines : list (ref string) -> ML unit
-let rec print_lines rs' = match rs' with
-  | [] -> ()
-  | (r::rs) -> print_string !r; print_string "\n"; print_lines rs
+type editorChar = (char * bool)
 
-val print_buffer : unit -> ML unit
-let print_buffer () =
-  print_lines !buffer
+val pad_line : nat -> list editorChar -> Tot (list editorChar)
+let pad_line n cs = pad_list n (' ',false) cs
 
-val handle_key : char -> ML unit
-let handle_key ch =
-  insert_char ch
+val isLineBreak : editorChar -> Tot bool
+let isLineBreak (ch,_) = (ch = '\n')
+
+val listLines : list editorChar -> Tot (list editorChar * list (list editorChar))
+let rec listLines cs' = match cs' with
+  | [] -> ([],[])
+  | c::cs -> let (line,lines) = listLines cs in
+    if isLineBreak c then
+      ([c], line :: lines)
+    else
+      (c::line, lines)
+
+val annotate : list char -> int -> Tot (list editorChar)
+let rec annotate cs' n = match cs' with
+  | [] -> []
+  | c::cs -> (c,n=0)::annotate cs (n-1)
+
+val scrubCursor : list (list editorChar) -> Tot (list (list char))
+let scrubCursor = map (map fst)
+
+val findCursorRow : list editorChar -> Tot (option nat)
+let rec findCursorRow es' = match es' with
+  | [] -> None
+  | (_,c)::es -> if c then Some 0 else
+    match (findCursorRow es) with
+      | None -> None
+      | Some n -> Some (n+1)
+
+val findCursor : list (list editorChar) -> Tot (option (nat * nat))
+let rec findCursor ess' = match ess' with
+  | [] -> None
+  | es::ess -> match findCursorRow es with
+    | Some n -> Some (0,n)
+    | None -> match findCursor ess with
+      | None -> None
+      | Some (m,n) -> Some (m+1,n)
+
+val findCursorOrZero : list (list editorChar) -> Tot (nat * nat)
+let findCursorOrZero ess = match findCursor ess with
+  | None -> (0,0)
+  | Some (m,n) -> (m,n)
+
+val display_buffer : buffer -> Tot terminalScreen
+let display_buffer (w, h, pos, bufstr) =
+  let echars = annotate bufstr pos in
+  let (line,lines) = listLines echars in
+  let lines' = line::lines in
+  let padded_lines = map (fun line -> pad_line w line) lines' in
+  let empty_line = pad_line w [] in
+  let egrid = pad_list h empty_line padded_lines in
+  let grid = scrubCursor egrid in
+  let (cx,cy) = findCursorOrZero egrid in
+  Screen w h cx cy grid
+
+type buffer_changer b =
+  p:(buffer * list char){Some (display_buffer (fst p)) = screen_advance (snd p) (display_buffer b)}
+//type buffer_changer (b:buffer) = (buffer * list char)
+
+//val l_screen_advance_empty : (s:terminalScreen) -> Lemma (screen_advance [] s = Some s)
+//let l_screen_advance_empty b = ()
+
+val state : ref buffer
+let state = ST.alloc (80,25,0,[])
+
+val noop : b:buffer -> Tot (buffer_changer b)
+let noop buf = (buf,[])
+
+val list_insert : nat -> 'a -> list 'a -> Tot (list 'a)
+let rec list_insert i y xs' =
+  match i with
+  | 0 -> y::xs'
+  | _ -> match xs' with
+    | [] -> [y]
+    | x::xs -> x::list_insert (i-1) y xs
+
+val insert_char : char -> b:buffer -> Tot (buffer_changer b)
+let insert_char ch (w,h,i,chars) =
+  let chars' = list_insert i ch chars in
+  let buf' = (w,h,i+1,chars') in
+  let output = esc::'['::'@'::ch::[] in
+  (buf', output)
+
+val handle_key : char -> b:buffer -> Tot (buffer_changer b)
+let handle_key ch buf =
+  if isPrintableChar ch then
+    insert_char ch buf
+  else
+    noop buf
 
 val editor : unit -> ML unit
 let rec editor () =
-  let ch = input_char () in
-  handle_key ch;
-  print_buffer ();
+  let (ch:char) = input_char () in
+  let (s:buffer) = !state in
+  let bch = handle_key ch s in
+  let (state', cs) = bch in
+  state := state';
+  print_string (charsstr cs);
   editor ()
 ;;
    
