terminal.fst
@@ -1,11 +1,17 @@
 (*--build-config
 options:--admit_fsi FStar.Set;
-other-files:set.fsi heap.fst st.fst all.fst io.fsti string.fst list.fst char.fst;
+other-files:set.fsi heap.fst st.fst all.fst io.fsti string.fst listTot.fst char.fst;
 --*)
 module Terminal
 
-open FStar.List
+open FStar.List.Tot
 open FStar.Char
+open FStar.String
+
+let op_At_At (xs:list 'a) (ys:list 'a) = append xs ys
+
+val charsstr : list char -> Tot string
+let charsstr cs = fold_right (fun c str -> strcat str (make 1 c)) cs ""
 
 val listmod : nat -> ('a -> Tot 'a) -> list 'a -> Tot (list 'a)
 let rec listmod n f xs' = match xs' with
@@ -20,7 +26,7 @@ let gridWith x y c g =
 
 type terminalState : Type =
   | StateDefault : terminalState
-  | StateEscape : string -> terminalState
+  | StateEscape : list char -> terminalState
 
 type terminalScreen : Type =
   | Screen :
@@ -36,6 +42,9 @@ type terminal : Type = option (terminalState * terminalScreen)
 val isPrintableChar : char -> Tot bool
 let isPrintableChar ch =
   (int_of_char ch >= int_of_char ' ') && (int_of_char ch <= int_of_char '~')
+
+val esc : char
+let esc = char_of_byte 27
 
 val screenPrint : char -> terminalScreen -> Tot (option terminalScreen)
 let screenPrint ch (Screen w h cx cy chars) =
@@ -63,16 +72,50 @@ let screenNop screen = Some screen
 val screenError : terminalScreen -> Tot (option terminalScreen)
 let screenError screen = None
 
+val init : list 'a -> Tot (list 'a)
+let rec init xs' = match xs' with
+  | [] -> []
+  | [x] -> []
+  | x::xs -> x::init xs
+
+val listins : list 'a -> nat -> 'a -> Tot (list 'a)
+let rec listins xs' n y = match xs' with
+  | [] -> []
+  | x::xs -> match n with
+    | 0 -> y::init xs'
+    | _ -> x::listins xs (n-1) y
+
+val screenInsertChar : char -> terminalScreen -> Tot (option terminalScreen)
+let screenInsertChar ch (Screen w h cx cy chars) =
+  let chars' = listmod cy (fun row -> listins row cx ch) chars in
+  Some (Screen w h cx cy chars')
+
+val screenDoEscape : list char -> terminalScreen -> Tot (option terminalScreen)
+let screenDoEscape str screen =
+  match charsstr str with
+    | "[@" -> screenInsertChar ' ' screen
+    | _ -> None
+
+val endsEscape : char -> Tot bool
+let endsEscape ch = (int_of_char ch >= int_of_char '@') && (int_of_char ch <= int_of_char 'Z')
+
 val termCharAction : char -> terminalState -> Tot ((terminalScreen -> Tot (option terminalScreen)) * terminalState)
 let termCharAction ch state =
-  if isPrintableChar ch && state = StateDefault then
-    (screenPrint ch, StateDefault)
-  else if ch = '\n' && state = StateDefault then
-    (screenNextLine, StateDefault)
-  else if ch = '\n' && state = StateDefault then
-    (screenNop, StateEscape "")
-  else
-    (screenError, StateDefault)
+  match state with
+    | StateDefault ->
+      if isPrintableChar ch && state = StateDefault then
+        (screenPrint ch, StateDefault)
+      else if ch = '\n' && state = StateDefault then
+        (screenNextLine, StateDefault)
+      else if ch = esc && state = StateDefault then
+        (screenNop, StateEscape [])
+      else
+        (screenError, StateDefault)
+    | StateEscape str ->
+       if endsEscape ch then
+         (screenDoEscape (str @@ [ch]), StateDefault)
+       else
+	 (screenNop, StateEscape (str @@ [ch]))
 
 val termChar : char -> terminal -> Tot terminal
 let termChar ch term =
@@ -85,3 +128,21 @@ let termChar ch term =
       | None -> None
     )
   | None -> None
+
+val weaken : n:nat -> m:nat{m<n} -> Tot (m':nat{m'<n+1})
+let weaken _ m = m
+
+val countUpTo : m:nat -> Tot (list (k:nat{k<m}))
+let rec countUpTo n = match n with
+  | 0 -> []
+  | _ -> map (weaken (n-1)) (countUpTo (n-1)) @@ [n-1]
+
+val strchars : string -> Tot (list char)
+let strchars str = map (fun i -> getTot str i) (countUpTo (strlen str))
+
+val termString : string -> terminal -> Tot terminal
+let termString str term =
+  fold_right termChar (strchars str) term
+
+val termChars : list char -> terminal -> Tot terminal
+let termChars cs term = fold_right termChar cs term
