Makefile
@@ -3,10 +3,11 @@ BIN=$(FSTAR_HOME)/bin
 FSTAR=$(BIN)/fstar.exe
 
 ADMIT=--admit_fsi FStar.Set --admit_fsi FStar.Heap --admit_fsi FStar.ST --admit_fsi FStar.All --admit_fsi FStar.IO
-LIBFILES=set.fsi heap.fst st.fst all.fst io.fsti string.fst list.fst char.fst
+LIBFILES=set.fsi heap.fst st.fst all.fst io.fsti string.fst listTot.fst char.fst
 
+#	$(FSTAR) --odir out --codegen OCaml $(ADMIT) $(LIBFILES) terminal.fst hello.fst
 ocaml: out hello.fst
-	$(FSTAR) --odir out --codegen OCaml $(ADMIT) $(LIBFILES) terminal.fst hello.fst
+	$(FSTAR) --odir out --codegen OCaml --use_build_config hello.fst
 	cp $(LIB)/ml/prims.ml $(LIB)/ml/FStar_IO.ml $(LIB)/ml/FStar_ST.ml $(LIB)/ml/FStar_String.ml $(LIB)/ml/FStar_List.ml out
 	(cd out; ocamlfind ocamlc -o hello.exe -package batteries -linkpkg prims.ml FStar_IO.ml FStar_ST.ml FStar_List.ml FStar_String.ml Hello.ml)
 	stty -echo -icanon
